theories/FOL/PrefixVocabulary/SuccCanonical.v
@@ -1,0 +1,11 @@
+(* Canonical model for [∃ ∧ ∀∃∀] formulas and their un-Skolemized form. *)
+
+(* In this file, we prove that given quantifier-free formulas
+   F(x, x', y) and Z(z), the following are equivalent:
+   (i)  Z(0) ∧ ∀x y. F(x, x+1, y) is satisfiable over the natural numbers
+   (ii) ∃z Z(z) ∧ ∀x ∃x' ∀y. F(x, x', y) is satisfiable over any model
+*)
+
+From Undecidability.FOL Require Import FullSyntax.
+
+
