theories/FOL/Utils/FriedmanValidity.v
@@ -1,0 +1,77 @@
+(* Validity of Friedman translation of Prenex formulas in decidable models. *)
+
+From Undecidability.FOL Require Import FullSyntax FriedmanTranslation PrenexNormalForm.
+Require Import Undecidability.Synthetic.DecidabilityFacts.
+Require Import Undecidability.Shared.Dec.
+
+
+Section FixModel.
+  Context {Σ_funcs : funcs_signature}.
+  Context {Σ_preds : preds_signature}.
+  Definition interp_dec {D} (I : interp D) := (forall p, decidable (fun v => i_atom (P:=p) v)).
+
+  Context {D : Type} {I : interp D}.
+  Hypothesis atom_dec : interp_dec I.
+
+  Lemma noQuant_dec_sat `{ff : falsity_flag} (rho : env D) {phi : form} :
+    noQuant_ind phi -> inhabited (dec (rho ⊨ phi)).
+  Proof using atom_dec.
+    intros H. induction H as [| | ff op phi1 phi2 H1 IH1 H2 IH2].
+    - constructor. exact False_dec.
+    - cbn.
+      specialize (atom_dec P).
+      apply decidable_iff in atom_dec.
+      destruct atom_dec as [P_dec].
+      constructor. apply P_dec.
+    - destruct IH1 as [IH1]. destruct IH2 as [IH2].
+      destruct op; constructor; cbn.
+      + apply and_dec; easy.
+      + apply or_dec; easy.
+      + apply impl_dec; easy.
+  Qed.
+
+  Local Instance I' : @interp Σ_funcs extended_preds D := extend_interp I False.
+
+  Lemma noQuant_Fr_iff `{ff : falsity_flag} (rho : env D) (phi : form) :
+    noQuant_ind phi -> rho ⊨ phi <-> rho ⊨ Fr phi.
+  Proof using atom_dec.
+    intros H. induction H as [| | ff' op phi1 phi2 H1 IH1 H2 IH2].
+    - (* falsity *) firstorder.
+    - (* atom *)
+      split; [firstorder|].
+      specialize (atom_dec P).
+      apply decidable_iff in atom_dec.
+      destruct atom_dec as [P_dec].
+      destruct (P_dec (Vector.map (eval rho) v)); firstorder.
+    - destruct op.
+      1,3: (* and, impl *) firstorder.
+      split; [firstorder|].
+      destruct (noQuant_dec_sat rho H1) as [[]];
+        destruct (noQuant_dec_sat rho H2) as [[]];
+        firstorder.
+  Qed.
+
+  Lemma PNF_Fr_sat `{ff : falsity_flag} (rho : env D) (phi : form) :
+    PNF_ind phi -> rho ⊨ phi -> rho ⊨ Fr phi.
+  Proof using atom_dec.
+    intros H. revert rho. induction H as [| ff op phi H IH]; intros rho.
+    - apply noQuant_Fr_iff, H.
+    - destruct op; firstorder.
+  Qed.
+
+  Lemma PNF_conj_Fr_sat `{ff : falsity_flag} (rho : env D) (phi : form) :
+    PNF_conj phi -> rho ⊨ phi -> rho ⊨ Fr phi.
+  Proof using atom_dec.
+    intros H. induction H.
+    - auto using PNF_Fr_sat.
+    - firstorder.
+  Qed.
+
+  Lemma PNF_conj_neg_Fr_sat (rho : env D) (phi : form) :
+    PNF_conj phi -> rho ⊨ Fr (¬ phi) -> rho ⊨ ¬ phi.
+  Proof using atom_dec.
+    intros Hpnf Hfr Hphi.
+    simpl in Hfr. apply Hfr.
+    now apply PNF_conj_Fr_sat.
+  Qed.
+End FixModel.
