theories/FOL/Utils/QuantifierPrefix.v
@@ -1,42 +1,106 @@
 From Undecidability.FOL Require Import FullSyntax PrenexNormalForm.
 From Stdlib Require Import ssrbool.
 
-Abbreviation quant := full_logic_quant.
+Abbreviation Quant := full_logic_quant.
 
 Import List ListNotations.
 
 Section QuantifierPrefix.
   Context {Σ_funcs : funcs_signature}.
   Context {Σ_preds : preds_signature}.
-  Context {ff : falsity_flag}.
 
-  Inductive quant_repeat :=
-    | unlimited (q : quant)
-    | once (q : quant).
+  Inductive qrep :=
+    | unlimited (q : Quant)
+    | once (q : Quant).
 
-  Definition quant_pattern := list quant_repeat.
+  Definition qpat := list qrep.
 
-  Declare Custom Entry qpat.
-  Declare Custom Entry qrep.
+  Fixpoint prefix {ff : falsity_flag} (phi : form) : list Quant :=
+    match phi with
+    | falsity => []
+    | atom _ _ => []
+    | bin _ _ _ => []
+    | quant q phi' => q :: prefix phi'
+    end.
+
+  Inductive matches_qpat : list Quant -> qpat -> Prop :=
+    | qNil           : matches_qpat nil nil
+    | qSkip q qs pat :
+        matches_qpat qs pat ->
+        matches_qpat qs (q :: pat)
+    | qOnce q qs pat :
+        matches_qpat qs pat ->
+        matches_qpat (q :: qs) (once q :: pat)
+    | qUnlimited q qs pat :
+        matches_qpat qs        (unlimited q :: pat) ->
+        matches_qpat (q :: qs) (unlimited q :: pat).
+
+  Definition PrefixClass {ff : falsity_flag} (pat : qpat) (phi : form) :=
+    closed phi /\ PNF_ind phi /\ matches_qpat (prefix phi) pat.
+
+  (* We generalize the notion of a quantifier prefix to the class to
+   * specify classes of conjunctions whose each clause has a specified
+   * quantifier prefix. This is useful for describing some of the intermediate
+   * classes that crop up in the classification of prefix-vocabulary classes. *)
+  Definition gpat := list qpat.
+
+  Fixpoint matches_gpat (prefs : list (list Quant)) (pats : gpat) : Prop :=
+    match prefs, pats with
+    | qs :: prefs, pat :: pats => matches_qpat qs pat /\ matches_gpat prefs pats
+    | _ :: _, [] => False
+    | [], _ => True
+    end.
+
+  Definition GPrefixClass {ff : falsity_flag} (pat : gpat) (phi : form) :=
+    closed phi /\ PNF_conj phi /\ matches_gpat (map prefix (unconj phi)) pat.
+
   Declare Custom Entry quant.
   Notation "'All'" := All (in custom quant at level 0).
   Notation "'Ex'" := Ex (in custom quant at level 0).
   Notation "∀" := All (in custom quant at level 0).
   Notation "∃" := Ex (in custom quant at level 0).
 
-  Notation "[ 'prefix' p ]" := p (p custom qpat, format "[ prefix  p ]").
+  Declare Custom Entry qrep.
   Notation "q *" := (unlimited q)
     (in custom qrep at level 1, q custom quant, format "q *").
   Notation "q" := (once q) (in custom qrep at level 1, q custom quant).
+
+  Declare Custom Entry qpat.
+  Notation "q ^ k qs" := (repeat q k ++ qs)
+    (in custom qpat at level 2, right associativity, q custom qrep,
+      k constr at level 100, format "q ^ k  qs").
   (* specify the type explicitly to make the pretty-printer work correctly *)
-  Notation "q qs" := (@cons quant_repeat q qs)
+  Notation "q qs" := (@cons qrep q qs)
     (in custom qpat at level 2, right associativity, q custom qrep).
-  Notation "q" := [q]
-    (in custom qpat at level 2, right associativity, q custom qrep).
+  Notation "" := (@nil qrep)
+    (in custom qpat at level 2, right associativity).
 
-  Notation "( x )" := x (in custom qpat, x at level 10).
-  Notation "{ x }" := x (in custom qpat, x constr).
+  (* pretty-printer special cases to avoid extraneous whitespace at the end *)
+  Notation "q" := (@cons qrep q (@nil qrep))
+    (in custom qpat at level 2, q custom qrep, only printing).
+  Notation "q ^ k" := (repeat q k ++ (@nil qrep))
+    (in custom qpat at level 2, q custom qrep, k constr at level 100,
+      format "q ^ k", only printing).
 
+  Declare Custom Entry gpat.
+  Notation "p" := (@cons qpat p (@nil qpat))
+    (in custom gpat at level 1, p custom qpat).
+  Notation "p ∧ ps" := (@cons qpat p ps)
+    (in custom gpat at level 1, right associativity, p custom qpat).
+  Notation "p /\ ps" := (@cons qpat p ps)
+    (in custom gpat at level 1, right associativity, p custom qpat,
+     only parsing).
+  Notation "[ 'prefix' p ]" := p (p custom qpat, format "[ prefix  p ]").
+  Notation "[ 'gprefix' p ]" := p (p custom gpat, format "[ gprefix  p ]").
+
+  (*
   Check [prefix ∀].
   Check [prefix ∀* ∃].
-  Check [prefix ∀* ∃ ∀*].
+  Check [prefix ∀* ∃^2 ∀*].
+  Check [prefix ∀* ∃^2].
+  Check []. (* make sure this doesn't get printed using the new notations *)
+
+  Check [gprefix ∀* ∃^2 ∀*].
+  Check [gprefix ∃ ∧ ∀∃∀].
+   *)
+End QuantifierPrefix.
